semantics/primTypesScript.sml
@@ -54,7 +54,7 @@ val _ = Define `
  ((prim_sem_env:'ffi ffi_state ->('ffi state#(v)sem_env)option) ffi=
    (add_to_sem_env
     (<| clock :=(( 0 : num)); ffi := ffi; refs := ([]); next_type_stamp :=(( 0 : num)); next_exn_stamp :=(( 0 : num));
-        fp_state := (<| rws := ([]); opts := no_fp_opts; canOpt := F; choices :=(( 0 : num));
+        fp_state := (<| rws := ([]); opts := no_fp_opts; canOpt := Strict; choices :=(( 0 : num));
                       assertions := no_assertions; real_sem := F |>) |>,
      <| v := nsEmpty; c := nsEmpty |>)
         prim_types_program))`;
