semantics/proofs/primSemEnvScript.sml
@@ -19,7 +19,7 @@ val _ = new_theory "primSemEnv";
 val prim_sem_env_eq = save_thm ("prim_sem_env_eq",
 ``add_to_sem_env (<| clock := 0; ffi := (ffi:'ffi ffi_state); refs := [];
                      next_exn_stamp := 0; next_type_stamp := 0;
-                     fp_state := <| rws := []; opts := no_fp_opts; canOpt := F;
+                     fp_state := <| rws := []; opts := no_fp_opts; canOpt := Strict;
                                     choices := 0; assertions := no_assertions;
                                     real_sem := F |> |>,
                   <| c := nsEmpty; v := nsEmpty |>)
